add stlc/lngen typing

stlc/lngen/def_ott.v
@@ -9,10 +9,12 @@ Definition expvar : Set := var.
 Inductive exp : Set := 
  | exp_var_b (_:nat)
  | exp_var_f (x:expvar)
+ | exp_unit : exp
  | exp_abs (e:exp)
  | exp_app (e1:exp) (e2:exp).
 
 Inductive typ : Set := 
+ | typ_unit : typ
  | typ_arr (A1:typ) (A2:typ).
 
 (* EXPERIMENTAL *)
@@ -30,6 +32,7 @@ Fixpoint open_exp_wrt_exp_rec (k:nat) (e_5:exp) (e__6:exp) {struct e__6}: exp :=
         | inright _ => exp_var_b (nat - 1)
       end
   | (exp_var_f x) => exp_var_f x
+  | exp_unit => exp_unit 
   | (exp_abs e) => exp_abs (open_exp_wrt_exp_rec (S k) e_5 e)
   | (exp_app e1 e2) => exp_app (open_exp_wrt_exp_rec k e_5 e1) (open_exp_wrt_exp_rec k e_5 e2)
 end.
@@ -43,6 +46,8 @@ Definition open_exp_wrt_exp e_5 e__6 := open_exp_wrt_exp_rec 0 e__6 e_5.
 Inductive lc_exp : exp -> Prop :=    (* defn lc_exp *)
  | lc_exp_var_f : forall (x:expvar),
      (lc_exp (exp_var_f x))
+ | lc_exp_unit : 
+     (lc_exp exp_unit)
  | lc_exp_abs : forall (e:exp),
       ( forall x , lc_exp  ( open_exp_wrt_exp e (exp_var_f x) )  )  ->
      (lc_exp (exp_abs e))
@@ -55,6 +60,7 @@ Fixpoint var_in_exp (e_5:exp) : vars :=
   match e_5 with
   | (exp_var_b nat) => {}
   | (exp_var_f x) => {{x}}
+  | exp_unit => {}
   | (exp_abs e) => (var_in_exp e)
   | (exp_app e1 e2) => (var_in_exp e1) \u (var_in_exp e2)
 end.
@@ -64,6 +70,7 @@ Fixpoint subst_exp_in_exp (e_5:exp) (x5:expvar) (e__6:exp) {struct e__6} : exp :
   match e__6 with
   | (exp_var_b nat) => exp_var_b nat
   | (exp_var_f x) => (if eq_var x x5 then e_5 else (exp_var_f x))
+  | exp_unit => exp_unit 
   | (exp_abs e) => exp_abs (subst_exp_in_exp e_5 x5 e)
   | (exp_app e1 e2) => exp_app (subst_exp_in_exp e_5 x5 e1) (subst_exp_in_exp e_5 x5 e2)
 end.
