stlc/lngen/def_extra.v
@@ -1,0 +1,38 @@
+Require Import stlc.lngen.def_ott.
+Require Import stlc.lngen.prop_ln.
+
+Definition ctx := list (atom * typ).
+
+Reserved Notation "Γ ⊢ t : A" 
+  (at level 99, t at next level, no associativity).
+Inductive typing : ctx -> exp -> typ -> Prop :=
+| typing_var : forall (Γ : ctx) (x : atom) (A : typ),
+  binds x A Γ ->
+  Γ ⊢ (exp_var_f x) : A
+| typing_unit : forall (Γ : ctx),
+  Γ ⊢ exp_unit : typ_unit
+| typing_abs : forall (L : atoms) (Γ : ctx) (A B : typ) (t : exp),
+  (forall x, 
+    x `notin` L -> ((x , A) :: Γ) ⊢ t : B) ->
+  Γ ⊢ (exp_abs t) : (typ_arr A B)
+| typing_app : forall (Γ : ctx) (s t : exp) (A B : typ),
+  Γ ⊢ s : (typ_arr A B) ->
+  Γ ⊢ t : A ->
+  Γ ⊢ (exp_app s t) : B
+where "Γ ⊢ t : A" := (typing Γ t A).
+
+Reserved Notation "t ⤳ t'" (at level 80).
+Inductive step : exp -> exp -> Prop :=
+| step_beta : forall (t s : exp),
+  exp_app (exp_abs t) s ⤳ open_exp_wrt_exp t s
+| step_app : forall (t t' s : exp),
+  t ⤳ t' ->
+  exp_app t s ⤳ exp_app t' s
+where "t ⤳ t'" := (step t t').
+
+Definition is_value (t : exp) : Prop :=
+  match t with
+  | exp_abs _ => True
+  | exp_unit => True
+  | _ => False
+  end.
