stlc/lngen/prop_typing.v
@@ -1,0 +1,37 @@
+Require Import stlc.lngen.def_ott.
+Require Import stlc.lngen.prop_ln.
+Require Import stlc.lngen.def_extra.
+
+Require Import Coq.Program.Equality.
+
+Hint Constructors typing : core.
+
+Theorem typing_subst Γ1 Γ2 x s t A B:
+  x `notin` dom (Γ2 ++ Γ1) ->
+  Γ2 ++ (x, B) :: Γ1 ⊢ t : A ->
+  Γ1 ⊢ s : B ->
+  Γ2 ++ Γ1 ⊢ (subst_exp_in_exp s x t) : A.
+Proof.
+  intros. dependent induction H0; eauto.
+  - simpl. destruct (x0 == x). admit.
+  - admit.
+  - simpl. eapply typing_app; eauto.
+Admitted.
+
+Corollary typing_subst0 Γ x s t A B: 
+  ((x, B) :: Γ) ⊢ t : A ->
+  Γ ⊢ s : B ->
+  Γ ⊢ (subst_exp_in_exp s x t) : A.
+Proof.
+  intros. rewrite <- (app_nil_l Γ). eapply typing_subst; eauto.
+Qed.
+
+Theorem preservation Γ t t' A : 
+  Γ ⊢ t : A ->
+  t ⤳ t' ->
+  Γ ⊢ t' : A.
+Proof.
+  intros Htyping Hstep. generalize dependent A.
+  induction Hstep; intros; inversion Htyping; subst; eauto.
+  - inversion H2. subst. admit.
+Admitted.
